theories/ftlr/Get.v
@@ -31,10 +31,11 @@ Section fundamental.
   Implicit Types interp : (D).
 
   Lemma get_case (W : WORLD) (C : CmptName) (regs : leibnizO Reg) (p p' : Perm)
-        (g : Locality) (b e a : Addr) (w : Word) (ρ : region_type) (dst r : RegName) (ins: instr) (P:D) (cstk : CSTK) (Ws : list WORLD) (wstk : Word)
+        (g : Locality) (b e a : Addr) (w : Word) (ρ : region_type) (dst r : RegName) (ins: instr)
+        (P:D) (cstk : CSTK) (Ws : list WORLD) (Cs : list CmptName) (wstk : Word)
         (Nswitcher : namespace) :
     is_Get ins dst r →
-    ftlr_instr W C regs p p' g b e a w ins ρ P cstk Ws wstk Nswitcher.
+    ftlr_instr W C regs p p' g b e a w ins ρ P cstk Ws Cs wstk Nswitcher.
   Proof.
     intros Hinstr Hp Hsome i Hbae Hfp HO Hpers Hpwl Hregion Hnotrevoked Hi.
     iIntros "#IH #Hinv_interp #Hreg #Hinva #Hrcond #Hwcond #Hmono #HmonoV Hw Hcont %Hframe Hsts Hown Htframe".
@@ -59,7 +60,7 @@ Section fundamental.
 
       assert (is_Some (<[dst:=WInt z]> (<[PC:=WCap x x0 x1 x2 x3]> regs) !! csp)) as [??].
       { destruct (decide (dst = csp)); simplify_map_eq=>//. }
-      iApply ("IH" $! _ _ _ _ (<[dst := _]> (<[PC := _]> regs))
+      iApply ("IH" $! _ _ _ _ _ (<[dst := _]> (<[PC := _]> regs))
                with "[%] [] [Hmap] [%] [$Hr] [$Hsts] [$Hcont] [//] [$Hown] [$Htframe]")
         ; eauto.
       + intro; cbn. by repeat (rewrite lookup_insert_is_Some'; right).
