theories/ftlr/ReadSR.v
@@ -33,9 +33,9 @@ Section fundamental.
 
   Lemma readsr_case (W : WORLD) (C : CmptName) (regs : leibnizO Reg)
     (p p' : Perm) (g : Locality) (b e a : Addr)
-    (w : Word) (ρ : region_type) (dst : RegName) (src : SRegName) (P:D) (cstk : CSTK) (Ws : list WORLD) (wstk : Word)
+    (w : Word) (ρ : region_type) (dst : RegName) (src : SRegName) (P:D) (cstk : CSTK) (Ws : list WORLD) (Cs : list CmptName) (wstk : Word)
     (Nswitcher : namespace) :
-    ftlr_instr W C regs p p' g b e a w (ReadSR dst src) ρ P cstk Ws wstk Nswitcher.
+    ftlr_instr W C regs p p' g b e a w (ReadSR dst src) ρ P cstk Ws Cs wstk Nswitcher.
   Proof.
     intros Hp Hsome HcorrectPC Hbae Hfp HO Hpers Hpwl Hregion Hnotrevoked Hi.
     iIntros "#IH #Hinv_interp #Hreg #Hinva #Hrcond #Hwcond #Hmono #HmonoV Hw Hcont %Hframe Hsts Hown Htframe".
