theories/ftlr/Restrict.v
@@ -55,9 +55,9 @@ Section fundamental.
 
   Lemma restrict_case (W : WORLD) (C : CmptName) (regs : leibnizO Reg)
     (p p' : Perm) (g : Locality) (b e a : Addr)
-    (w : Word) (ρ : region_type) (dst : RegName) (src : Z + RegName) (P:D) (cstk : CSTK) (Ws : list WORLD) (wstk : Word)
+    (w : Word) (ρ : region_type) (dst : RegName) (src : Z + RegName) (P:D) (cstk : CSTK) (Ws : list WORLD) (Cs : list CmptName) (wstk : Word)
     (Nswitcher : namespace) :
-    ftlr_instr W C regs p p' g b e a w (Restrict dst src) ρ P cstk Ws wstk Nswitcher.
+    ftlr_instr W C regs p p' g b e a w (Restrict dst src) ρ P cstk Ws Cs wstk Nswitcher.
   Proof.
     intros Hp Hsome HcorrectPC Hbae Hfp HO Hpers Hpwl Hregion Hnotrevoked Hi.
     iIntros "#IH #Hinv_interp #Hreg #Hinva #Hrcond #Hwcond #Hmono #HmonoV Hw Hcont %Hframe Hsts Hown Htframe".
@@ -91,7 +91,7 @@ Section fundamental.
         destruct (executeAllowed p'') eqn:Hpft.
         {
           simplify_map_eq ; map_simpl "Hmap".
-          iApply ("IH" $! _ _ _ _ regs with "[%] [] [Hmap] [%] [$Hr] [$Hsts] [$Hcont] [//] [$Hown] [$Htframe]"); eauto.
+          iApply ("IH" $! _ _ _ _ _ regs with "[%] [] [Hmap] [%] [$Hr] [$Hsts] [$Hcont] [//] [$Hown] [$Htframe]"); eauto.
           iModIntro.
           iApply (PermPairFlows_interp_preserved); eauto.
           iApply (interp_next_PC with "Hinv_interp"); eauto.
@@ -109,7 +109,7 @@ Section fundamental.
         { destruct ρ;auto;contradiction. }
         assert (is_Some (<[dst:=WCap p'0 g' b0 e0 a0]> (<[PC:=WCap p'' g'' b'' e'' a'']> regs) !! csp)) as [??].
         { destruct (decide (dst = csp)); simplify_map_eq=>//. }
-        iApply ("IH" $! _ _ _ _ (<[dst:=_]> _) with "[%] [] [Hmap] [%] [$Hr] [$Hsts] [$Hcont] [//] [$Hown] [$Htframe]"); eauto.
+        iApply ("IH" $! _ _ _ _ _ (<[dst:=_]> _) with "[%] [] [Hmap] [%] [$Hr] [$Hsts] [$Hcont] [//] [$Hown] [$Htframe]"); eauto.
         - intros; simpl. repeat (rewrite lookup_insert_is_Some'; right); eauto.
         - iIntros (ri v Hri Hvs).
           destruct (decide (ri = dst)).
@@ -138,7 +138,7 @@ Section fundamental.
       simplify_map_eq; map_simpl "Hmap".
       assert (is_Some (<[dst:=WSealRange p'0 g' b0 e0 a0]> regs !! csp)) as [??].
       { destruct (decide (dst = csp)); simplify_map_eq=>//. }
-      iApply ("IH" $! _ _ _ _ (<[dst:=WSealRange p'0 g' b0 e0 a0]> regs) with
+      iApply ("IH" $! _ _ _ _ _ (<[dst:=WSealRange p'0 g' b0 e0 a0]> regs) with
                "[%] [] [Hmap] [//] [$Hr] [$Hsts] [$Hcont] [//] [$Hown] [$Htframe]"); eauto.
       + intros. by rewrite lookup_insert_is_Some' ; right.
       + iIntros (ri v Hri Hvs).
